update

CellularAutomatas/proofs/exp_word_length_rt.lean
@@ -13,5 +13,88 @@ variable {α: Type u} [Alphabet α]
 variable {Γ: Type u} [Alphabet Γ]
 
 
+
+inductive ExpState
+| Init
+| FirstStep
+| Empty
+| Empty_Pos1
+| SignalRight
+| SignalLeft
+| Wall_S0
+| Wall_S1
+| Wall_S2
+| Wall_S3
+| Wall_S4
+| Collision
+| Collision_Pos1
+| Dead
+deriving DecidableEq, Repr, Fintype
+
+instance : Inhabited ExpState := ⟨ ExpState.Init ⟩
+
+def exp_ca : tCellAutomaton Unit := {
+  Q := ExpState,
+  δ := fun left center right =>
+    match center with
+    | ExpState.Init =>
+      match left with
+      | ExpState.Dead => ExpState.FirstStep
+      | ExpState.FirstStep => ExpState.Collision_Pos1
+      | ExpState.Wall_S0 => ExpState.Wall_S1
+      | ExpState.Collision => ExpState.Wall_S1
+      | ExpState.Collision_Pos1 => ExpState.Wall_S1
+      | _ => ExpState.Init
+    | ExpState.FirstStep => ExpState.Empty
+    | ExpState.Empty =>
+      if left == ExpState.SignalRight then ExpState.SignalRight
+      else if right == ExpState.SignalLeft || right == ExpState.Collision || right == ExpState.Collision_Pos1 then ExpState.SignalLeft
+      else if left == ExpState.Wall_S0 || left == ExpState.Collision then ExpState.Wall_S1
+      else ExpState.Empty
+    | ExpState.Empty_Pos1 =>
+      if left == ExpState.SignalLeft then ExpState.SignalRight
+      else if left == ExpState.SignalRight then ExpState.SignalRight
+      else if right == ExpState.SignalLeft || right == ExpState.Collision then ExpState.SignalLeft
+      else ExpState.Empty_Pos1
+    | ExpState.SignalRight => ExpState.Empty
+    | ExpState.SignalLeft =>
+      if left == ExpState.Dead then ExpState.Empty
+      else ExpState.Empty
+    | ExpState.Wall_S0 => ExpState.Empty
+    | ExpState.Wall_S1 =>
+      if left == ExpState.SignalRight then ExpState.Collision
+      else ExpState.Wall_S2
+    | ExpState.Wall_S2 =>
+      if left == ExpState.SignalRight then ExpState.Collision
+      else ExpState.Wall_S3
+    | ExpState.Wall_S3 =>
+      if left == ExpState.SignalRight then ExpState.Collision
+      else ExpState.Wall_S4
+    | ExpState.Wall_S4 =>
+      if left == ExpState.SignalRight then ExpState.Collision
+      else ExpState.Wall_S0
+    | ExpState.Collision => ExpState.Empty
+    | ExpState.Collision_Pos1 => ExpState.Empty_Pos1
+    | ExpState.Dead => ExpState.Dead,
+  border := ExpState.Dead,
+  p := fun n => 0,
+  t := fun n => n - 1,
+  embed := fun _ => ExpState.Init,
+  F_pos := fun q =>
+    match q with
+    | ExpState.Init => true
+    | ExpState.FirstStep => true
+    | ExpState.SignalLeft => true
+    | _ => false
+}
+
+
+#eval ((List.range 12).map (fun i => List.replicate i ())).map (fun w => decide (exp_ca.L w))
+  = [false, true, true, false, true, false, false, false, true, false, false, false]
+
 theorem exp_word_length_rt: ∃ C: CA_rt Unit, C.val.L = { w | ∃ n, w.length = 2 ^ n } := by
+  use ⟨ exp_ca, by simp [CA_rt, t_rt, CA, exp_ca, tCellAutomatons] ⟩
+  unfold tCellAutomaton.L
+  ext w
+  simp
   sorry
