CellularAutomatas/proofs/fsm_lemmas.lean
@@ -1,0 +1,22 @@
+import CellularAutomatas.defs
+import Mathlib.Data.List.Basic
+
+namespace fsm_lemmas
+
+def IdentityReconstructM (Q: Type u) [Alphabet Q]: FiniteStateMachine Q := {
+  Q := Q
+  δ := fun _ a => a
+  q0 := default
+}
+
+lemma scanr_identity (Q: Type u) [Alphabet Q] (w: Word Q):
+  (IdentityReconstructM Q).scanr w = w := by
+  simp [FiniteStateMachine.scanr, FiniteStateMachine.scanr_q]
+  induction w with
+  | nil => rfl
+  | cons a w ih =>
+    simp [FiniteStateMachine.scanr_step]
+    rw [ih]
+    cases w <;> simp [IdentityReconstructM]
+
+end fsm_lemmas
